fix add_and_double

code/curve25519/Hacl.Impl.Curve25519.AddAndDouble.fst
@@ -16,6 +16,7 @@ module F51 = Hacl.Impl.Curve25519.Field51
 module F64 = Hacl.Impl.Curve25519.Field64
 
 module P = Spec.Curve25519
+module S = Hacl.Spec.Curve25519.AddAndDouble
 
 #reset-options "--z3rlimit 150 --max_fuel 1 --using_facts_from '* -FStar.Seq'"
 
@@ -36,67 +37,45 @@ let fget_x (#s:field_spec) (h:mem) (p:point s) = feval h (gsub p 0ul (nlimb s))
 let fget_z (#s:field_spec) (h:mem) (p:point s) = feval h (gsub p (nlimb s) (nlimb s))
 let fget_xz (#s:field_spec) (h:mem) (p:point s) = fget_x h p, fget_z h p
 
-val point_tmp_inv_t:#s:field_spec -> h:mem -> f:felem s -> Type0
-let point_tmp_inv_t #s h f =
+val point_post_sub_t:#s:field_spec -> h:mem -> f:felem s -> Type0
+let point_post_sub_t #s h f =
   match s with
   | M51 -> F51.felem_fits h f (9, 10, 9, 9, 9)
+  | M64 -> True
+
+val point_post_add_t:#s:field_spec -> h:mem -> f:felem s -> Type0
+let point_post_add_t #s h f =
+  match s with
+  | M51 -> F51.felem_fits h f (2, 4, 2, 2, 2)
   | M64 -> True
 
 inline_for_extraction noextract
 val point_add_and_double0:
     #s:field_spec
-  -> q:point s
-  -> nq:point s
   -> nq_p1:point s
   -> ab:lbuffer (limb s) (2ul *! nlimb s)
   -> dc:lbuffer (limb s) (2ul *! nlimb s)
   -> tmp2:felem_wide2 s
   -> Stack unit
     (requires fun h0 ->
-      (s = M64 ==> X64.CPU_Features_s.(adx_enabled /\ bmi2_enabled)) /\    
-      live h0 q /\ live h0 nq /\ live h0 nq_p1 /\ live h0 ab /\ live h0 dc /\ live h0 tmp2 /\
-      disjoint q nq /\ disjoint q nq_p1 /\ disjoint q ab /\ disjoint q dc /\ disjoint q tmp2 /\
-      disjoint nq q /\ disjoint nq nq_p1 /\ disjoint nq ab /\ disjoint nq dc /\ disjoint nq tmp2 /\
+      (s = M64 ==> X64.CPU_Features_s.(adx_enabled /\ bmi2_enabled)) /\
+      live h0 nq_p1 /\ live h0 ab /\ live h0 dc /\ live h0 tmp2 /\
       disjoint nq_p1 ab /\ disjoint nq_p1 dc /\ disjoint nq_p1 tmp2 /\
       disjoint ab dc /\ disjoint ab tmp2 /\ disjoint dc tmp2 /\
-      state_inv_t h0 (get_x q) /\ state_inv_t h0 (get_z q) /\
-      state_inv_t h0 (get_x nq) /\ state_inv_t h0 (get_z nq) /\
       state_inv_t h0 (get_x nq_p1) /\ state_inv_t h0 (get_z nq_p1) /\
-      point_tmp_inv_t h0 (gsub ab 0ul (nlimb s)) /\
-      point_tmp_inv_t h0 (gsub ab (nlimb s) (nlimb s)) /\
-      feval h0 (gsub ab 0ul (nlimb s)) == P.fadd (fget_x h0 nq) (fget_z h0 nq) /\
-      feval h0 (gsub ab (nlimb s) (nlimb s)) == P.fsub (fget_x h0 nq) (fget_z h0 nq))
+      point_post_add_t h0 (gsub ab 0ul (nlimb s)) /\
+      point_post_sub_t h0 (gsub ab (nlimb s) (nlimb s)))
     (ensures  fun h0 _ h1 ->
       modifies (loc nq_p1 |+| loc dc |+| loc tmp2) h0 h1 /\
-      state_inv_t h1 (get_x nq_p1) /\ state_inv_t h1 (get_z nq_p1) /\
-      fget_xz h1 nq_p1 == P.add (fget_xz h0 q) (fget_xz h0 nq) (fget_xz h0 nq_p1))
-let point_add_and_double0 #s q nq nq_p1 ab dc tmp2 =
-  let x1 = sub q 0ul (nlimb s) in
-  let z1 = sub q (nlimb s) (nlimb s) in
-  let x2 = sub nq 0ul (nlimb s) in
-  let z2 = sub nq (nlimb s) (nlimb s) in
+      point_post_add_t h1 (get_x nq_p1) /\ point_post_sub_t h1 (get_z nq_p1) /\
+      fget_xz h1 nq_p1 == S.add_and_double1_0 (fget_x h0 ab) (fget_z h0 ab) (fget_xz h0 nq_p1))
+let point_add_and_double0 #s nq_p1 ab dc tmp2 =
   let x3 = sub nq_p1 0ul (nlimb s) in
   let z3 = sub nq_p1 (nlimb s) (nlimb s) in
   let a : felem s = sub ab 0ul (nlimb s) in
   let b : felem s = sub ab (nlimb s) (nlimb s) in
   let d : felem s = sub dc 0ul (nlimb s) in
   let c : felem s = sub dc (nlimb s) (nlimb s) in
-
-  let h0 = ST.get () in
-  assert (gsub q 0ul (nlimb s) == x1);
-  assert (gsub nq 0ul (nlimb s) == x2);
-  assert (gsub nq (nlimb s) (nlimb s) == z2);
-  assert (gsub nq_p1 0ul (nlimb s) == x3);
-  assert (gsub nq_p1 (nlimb s) (nlimb s) == z3);
-  assert (gsub ab 0ul (nlimb s) == a);
-  assert (gsub ab (nlimb s) (nlimb s) == b);
-  assert (gsub dc 0ul (nlimb s) == d);
-  assert (gsub dc (nlimb s) (nlimb s) == c);
-
-  //fadd a x2 z2; // a = x2 + z2
-  //fsub b x2 z2; // b = x2 - z2
-  assert (feval h0 a == P.fadd (feval h0 x2) (feval h0 z2));
-  assert (feval h0 b == P.fsub (feval h0 x2) (feval h0 z2));
 
   fadd c x3 z3; // c = x3 + z3
   fsub d x3 z3; // d = x3 - z3
@@ -106,39 +85,37 @@ let point_add_and_double0 #s q nq nq_p1 ab dc tmp2 =
   //fmul c c b;   // c = cb = c * b
   fmul2 dc dc ab tmp2;   // d|c = d*a|c*b
   fadd x3 d c;  // x3 = da + cb
-  fsub z3 d c;  // z3 = da - cb
-
-  //moving the following line gave me a 2k speedup.
-  (* CAN RUN IN PARALLEL *)
-  //fsqr x3 x3;   // x3 = (da + cb) ^ 2
-  //fsqr z3 z3;   // z3 = (da - cb) ^ 2
-  fsqr2 nq_p1 nq_p1 tmp2;   // x3|z3 = x3*x3|z3*z3
-  // moving the following line gives a 2k speedup
-  fmul z3 z3 x1 tmp2 // z3 = x1 * (da - cb) ^ 2
+  fsub z3 d c  // z3 = da - cb
 
 inline_for_extraction noextract
 val point_add_and_double1:
     #s:field_spec
   -> nq:point s
+  -> nq_p1:point s
   -> tmp1:lbuffer (limb s) (4ul *! nlimb s)
   -> tmp2:felem_wide2 s
   -> Stack unit
     (requires fun h0 ->
-      (s = M64 ==> X64.CPU_Features_s.(adx_enabled /\ bmi2_enabled)) /\    
-      live h0 nq /\ live h0 tmp1 /\ live h0 tmp2 /\
-      disjoint nq tmp1 /\ disjoint nq tmp2 /\ disjoint tmp1 tmp2 /\
+      (s = M64 ==> X64.CPU_Features_s.(adx_enabled /\ bmi2_enabled)) /\
+      live h0 nq /\ live h0 nq_p1 /\ live h0 tmp1 /\ live h0 tmp2 /\
+      disjoint nq nq_p1 /\ disjoint nq tmp1 /\ disjoint nq tmp2 /\
+      disjoint nq_p1 tmp1 /\ disjoint nq_p1 tmp2 /\ disjoint tmp1 tmp2 /\
       state_inv_t h0 (get_x nq) /\ state_inv_t h0 (get_z nq) /\
-      point_tmp_inv_t h0 (gsub tmp1 0ul (nlimb s)) /\
-      point_tmp_inv_t h0 (gsub tmp1 (nlimb s) (nlimb s)) /\
-      feval h0 (gsub tmp1 0ul (nlimb s)) == P.fadd (fget_x h0 nq) (fget_z h0 nq) /\
-      feval h0 (gsub tmp1 (nlimb s) (nlimb s)) == P.fsub (fget_x h0 nq) (fget_z h0 nq))
+      point_post_add_t h0 (gsub tmp1 0ul (nlimb s)) /\
+      point_post_sub_t h0 (gsub tmp1 (nlimb s) (nlimb s)) /\
+      point_post_add_t h0 (get_x nq_p1) /\ point_post_sub_t h0 (get_z nq_p1))
     (ensures  fun h0 _ h1 ->
-      modifies (loc nq |+| loc tmp1 |+| loc tmp2) h0 h1 /\
+      modifies (loc nq |+| loc nq_p1 |+| loc tmp1 |+| loc tmp2) h0 h1 /\
       state_inv_t h1 (get_x nq) /\ state_inv_t h1 (get_z nq) /\
-      fget_xz h1 nq == P.double (fget_xz h0 nq))
-let point_add_and_double1 #s nq tmp1 tmp2 =
+      state_inv_t h1 (get_x nq_p1) /\ state_inv_t h1 (get_z nq_p1) /\
+      (fget_xz h1 nq, fget_xz h1 nq_p1) ==
+	S.add_and_double1_1 (feval h0 (gsub tmp1 0ul (nlimb s)))
+	  (feval h0 (gsub tmp1 (nlimb s) (nlimb s))) (fget_xz h0 nq_p1))
+let point_add_and_double1 #s nq nq_p1 tmp1 tmp2 =
   let x2 = sub nq 0ul (nlimb s) in
   let z2 = sub nq (nlimb s) (nlimb s) in
+  let x3 = sub nq_p1 0ul (nlimb s) in
+  let z3 = sub nq_p1 (nlimb s) (nlimb s) in
 
   let a : felem s = sub tmp1 0ul (nlimb s) in
   let b : felem s = sub tmp1 (nlimb s) (nlimb s) in
@@ -147,23 +124,15 @@ let point_add_and_double1 #s nq tmp1 tmp2 =
 
   let ab : felem2 s = sub tmp1 0ul (2ul *! nlimb s) in
   let dc : felem2 s = sub tmp1 (2ul *! nlimb s) (2ul *! nlimb s) in
-  let h0 = ST.get () in
-  assert (gsub nq 0ul (nlimb s) == x2);
-  assert (gsub nq (nlimb s) (nlimb s) == z2);
-  assert (gsub ab 0ul (nlimb s) == a);
-  assert (gsub ab (nlimb s) (nlimb s) == b);
-  assert (gsub dc 0ul (nlimb s) == d);
-  assert (gsub dc (nlimb s) (nlimb s) == c);
-
-  //fadd a x2 z2; // a = x2 + z2
-  //fsub b x2 z2; // b = x2 - z2
-  assert (feval h0 a == P.fadd (feval h0 x2) (feval h0 z2));
-  assert (feval h0 b == P.fsub (feval h0 x2) (feval h0 z2));
-
   (* CAN RUN IN PARALLEL *)
   //fsqr d a;     // d = aa = a^2
   //fsqr c b;     // c = bb = b^2
   fsqr2 dc ab tmp2;     // d|c = aa | bb
+  (* CAN RUN IN PARALLEL *)
+  //fsqr x3 x3;   // x3 = (da + cb) ^ 2
+  //fsqr z3 z3;   // z3 = (da - cb) ^ 2
+  fsqr2 nq_p1 nq_p1 tmp2;   // x3|z3 = x3*x3|z3*z3
+
   copy_felem a c;                           // a = bb
   fsub c d c;   // c = e = aa - bb
   assert_norm (121665 < pow2 17);
@@ -183,7 +152,7 @@ val point_add_and_double_:
   -> tmp2:felem_wide2 s
   -> Stack unit
     (requires fun h0 ->
-      (s = M64 ==> X64.CPU_Features_s.(adx_enabled /\ bmi2_enabled)) /\    
+      (s = M64 ==> X64.CPU_Features_s.(adx_enabled /\ bmi2_enabled)) /\
     (
       let nq = gsub p01_tmp1 0ul (2ul *! nlimb s) in
       let nq_p1 = gsub p01_tmp1 (2ul *! nlimb s) (2ul *! nlimb s) in
@@ -201,33 +170,28 @@ val point_add_and_double_:
      (let p2, p3 = P.add_and_double (fget_xz h0 q) (fget_xz h0 nq) (fget_xz h0 nq_p1) in
       fget_xz h1 nq == p2 /\ fget_xz h1 nq_p1 == p3)))
 let point_add_and_double_ #s q p01_tmp1 tmp2 =
+  let h0 = ST.get () in
   let nq : point s = sub p01_tmp1 0ul (2ul *! nlimb s) in
   let nq_p1 : point s = sub p01_tmp1 (2ul *! nlimb s) (2ul *! nlimb s) in
   let tmp1 = sub p01_tmp1 (4ul *! nlimb s) (4ul *! nlimb s) in
 
+  let x1 = sub q 0ul (nlimb s) in
   let x2 = sub nq 0ul (nlimb s) in
   let z2 = sub nq (nlimb s) (nlimb s) in
+  let z3 = sub nq_p1 (nlimb s) (nlimb s) in
 
   let a : felem s = sub tmp1 0ul (nlimb s) in
   let b : felem s = sub tmp1 (nlimb s) (nlimb s) in
   let ab : felem2 s = sub tmp1 0ul (2ul *! nlimb s) in
   let dc : felem2 s = sub tmp1 (2ul *! nlimb s) (2ul *! nlimb s) in
 
-  assert (gsub p01_tmp1 0ul (2ul *! nlimb s) == nq);
-  assert (gsub p01_tmp1 (2ul *! nlimb s) (2ul *! nlimb s) == nq_p1);
-  assert (gsub p01_tmp1 (4ul *! nlimb s) (4ul *! nlimb s) == tmp1);
-  assert (gsub nq 0ul (nlimb s) == x2);
-  assert (gsub nq (nlimb s) (nlimb s) == z2);
-  assert (gsub ab 0ul (nlimb s) == a);
-  assert (gsub ab (nlimb s) (nlimb s) == b);
-  assert (gsub tmp1 0ul (2ul *! nlimb s) == ab);
-  assert (gsub tmp1 (2ul *! nlimb s) (2ul *! nlimb s) == dc);
-
   fadd a x2 z2; // a = x2 + z2
   fsub b x2 z2; // b = x2 - z2
 
-  point_add_and_double0 #s q nq nq_p1 ab dc tmp2;
-  point_add_and_double1 #s nq tmp1 tmp2
+  point_add_and_double0 #s nq_p1 ab dc tmp2;
+  point_add_and_double1 #s nq nq_p1 tmp1 tmp2;
+  fmul z3 z3 x1 tmp2; // z3 = x1 * (da - cb) ^ 2
+  S.lemma_add_and_double (fget_xz h0 q) (fget_xz h0 nq) (fget_xz h0 nq_p1)
 
 (* WRAPPER to Prevent Inlining *)
 [@CInline]
@@ -242,8 +206,8 @@ val point_add_and_double:
   -> p01_tmp1:lbuffer (limb s) (8ul *! nlimb s)
   -> tmp2:felem_wide2 s
   -> Stack unit
-    (requires fun h0 -> 
-      (s = M64 ==> X64.CPU_Features_s.(adx_enabled /\ bmi2_enabled)) /\    
+    (requires fun h0 ->
+      (s = M64 ==> X64.CPU_Features_s.(adx_enabled /\ bmi2_enabled)) /\
     (
       let nq = gsub p01_tmp1 0ul (2ul *! nlimb s) in
       let nq_p1 = gsub p01_tmp1 (2ul *! nlimb s) (2ul *! nlimb s) in
@@ -275,7 +239,7 @@ val point_double_:
   -> tmp2:felem_wide2 s
   -> Stack unit
     (requires fun h0 ->
-      (s = M64 ==> X64.CPU_Features_s.(adx_enabled /\ bmi2_enabled)) /\    
+      (s = M64 ==> X64.CPU_Features_s.(adx_enabled /\ bmi2_enabled)) /\
       live h0 nq /\ live h0 tmp1 /\ live h0 tmp2 /\
       disjoint nq tmp1 /\ disjoint nq tmp2 /\ disjoint tmp1 tmp2 /\
       state_inv_t h0 (get_x nq) /\ state_inv_t h0 (get_z nq))
@@ -334,7 +298,7 @@ val point_double:
   -> tmp2:felem_wide2 s
   -> Stack unit
     (requires fun h0 ->
-      (s = M64 ==> X64.CPU_Features_s.(adx_enabled /\ bmi2_enabled)) /\    
+      (s = M64 ==> X64.CPU_Features_s.(adx_enabled /\ bmi2_enabled)) /\
       live h0 nq /\ live h0 tmp1 /\ live h0 tmp2 /\
       disjoint nq tmp1 /\ disjoint nq tmp2 /\ disjoint tmp1 tmp2 /\
       state_inv_t h0 (get_x nq) /\ state_inv_t h0 (get_z nq))
